Toward SpMSpV (#15)
* port spvspv

* port spvspv

* progress

* progress

* ucsr spmspv

CSR.v
@@ -5,8 +5,8 @@ Require Export Relation_Definitions.
 Locate "_ ==> _ ==> _". Check Morphisms.respectful. *)
 
 From SLF Require Import LabType Fun LibSepFmap Sum.
-From SLF Require Import LibWP LibSepSimpl LibSepReference LibSepTLCbuffer.
-From SLF Require Import Struct Loops Unary_IndexWithBounds SV2 Subst NTriple Loops2 Struct2.
+From SLF Require Import LibWP LibSepSimpl LibSepReference LibSepTLCbuffer ListCommon.
+From SLF Require Import Struct Loops Unary_IndexWithBounds SV Subst NTriple Loops2 Struct2.
 From mathcomp Require Import ssreflect ssrfun zify.
 Hint Rewrite conseq_cons' : rew_listx.
 
@@ -108,12 +108,6 @@ Tactic Notation "seclocal_fold" :=
     -/(For_aux _ _) 
     -/(For _ _ _) //=.
 
-
-Lemma in_interval_list {A : Type} (l : list A) lb rb x: 
-   In x (list_interval lb rb l) -> In x l.
-Proof.
-Admitted.
-
 Arguments in_interval_list {_ _ _ _ _}.
 
 Local Notation Dom := (int * int)%type.
@@ -196,27 +190,6 @@ Definition spmv :=
   s
 }>.
 
-Lemma htriple_alloc0_unary {D : Type} `{Inhab D} (n : int) (d : D) :
-  htriple (single d tt) (fun=> alloc0 n)
-    \[0 <= n]
-    (fun hv => \exists p, \[hv = fun=> val_loc p] \* harray_fun (fun=> 0) p n d).
-(* Proof with fold'. *)
-  (* apply wp_equiv. xsimpl. intros HH.
-  assert (n = abs n :> int) as E by math.
-  rewrite -> E.
-  xwp; xapp (@htriple_alloc_nat)=>x p EE... rewrite !EE.
-  xwp; xapp (@htriple_memset0_unary). xwp; xval. xsimpl*.
-  rewrite -length_List_length length_make. xsimpl.
-Qed. *)
-Admitted.
-
-Add Parametric Morphism D : (@harray_fun D) with signature 
-  Morphisms.respectful (fun f g => forall x, f x = g x) (eq) as blah.
-Admitted.
-
-
-
-
 Lemma spmv_spec `{Inhab D} (x_mval x_colind x_rowptr x_dvec : loc) : 
   {{ arr(x_mval, mval)⟨1, (0,0)⟩ \*
      arr(x_colind, colind)⟨1, (0,0)⟩ \*
@@ -257,6 +230,87 @@ Proof with (try seclocal_fold; seclocal_solver).
     xapp @lhtriple_array_set_pre; try math.
     rewrite sum_prod1E; xsimpl. }
   { xwp; xval. xsimpl*. xsimpl; rewrite sum_prod1E; xsimpl. }
+Qed.
+
+Context (yind yval : list int).
+Context (M : int).
+Hypothesis len_xind : length yind = M :> int.
+Hypothesis len_xval : length yval = M :> int.
+Hypothesis stored_yind : sorted yind.
+Hypothesis yind_leq : forall x, In x yind -> 0 <= x < Ncol.
+Hypothesis Nrow0 : Nrow > 0. (* we get rid of it later *)
+
+
+Hypothesis sorted_eachcol : forall x : int, 0 <= x < Nrow -> sorted (colind_seg x).
+
+Definition spmspv x_colind y_ind x_mval y_val := 
+  let dot := sv.sv_dotprod x_colind y_ind x_mval y_val in
+  <{
+  fun rowptr =>
+  let s = alloc0 Nrow in
+  for i <- [0, Nrow] {
+    let lb = read_array rowptr i in
+    let i' = i + 1 in
+    let rb = read_array rowptr i' in
+    let x = dot lb rb 0 M in 
+      val_array_set s i x
+  }; 
+  s
+}>.
+
+Arguments Union_same {_ _} _ _.
+
+Lemma spmspv_spec `{Inhab D}
+  (x_mval x_colind x_rowptr y_ind y_val : loc) : 
+  {{ arr(x_mval, mval)⟨1, (0,0)⟩ \*
+     arr(x_colind, colind)⟨1, (0,0)⟩ \*
+     arr(x_rowptr, rowptr)⟨1, (0,0)⟩ \*
+     arr(y_ind, yind)⟨1, (0,0)⟩ \* 
+     arr(y_val, yval)⟨1, (0,0)⟩ \* 
+     (\*_(i <- `[0, Nrow] \x `[0, Ncol]) arr(x_mval, mval)⟨2, i⟩) \*
+     (\*_(i <- `[0, Nrow] \x `[0, Ncol]) arr(x_colind, colind)⟨2, i⟩) \*
+     (\*_(i <- `[0, Nrow] \x `[0, Ncol]) arr(x_rowptr, rowptr)⟨2, i⟩) \*
+     (\*_(i <- `[0, Ncol]) arr(y_ind, yind)⟨3, (0,i)⟩) \* 
+     (\*_(i <- `[0, Ncol]) arr(y_val, yval)⟨3, (0,i)⟩) }}
+  [{
+    {1| ld in `{(0,0)}                 => spmspv x_colind y_ind x_mval y_val x_rowptr};
+    {2| ld in `[0, Nrow] \x `[0, Ncol] => get x_mval x_colind x_rowptr ld.1 ld.2};
+    {3| ld in `{0}       \x `[0, Ncol] => sv.get ld.2 y_ind y_val 0 M}
+  }]
+  {{ hv, (\exists p, 
+    \[hv[`1]((0,0)) = val_loc p] \*
+    harray_fun (fun i => Σ_(j <- `[0, Ncol]) hv[`2]((i, j)) * hv[`3]((0, j))) p Nrow (Lab (1,0) (0,0)))
+      \* \Top }}. (* this \Top can be made concrete, if needed *)
+Proof with (try seclocal_fold; seclocal_solver; try lia).
+  xin (2,0) : do 3 (xwp; xapp).
+  xin (1,0) : (xwp; xapp (@htriple_alloc0_unary)=> // s)...
+  rewrite prod_cascade -(Union_same Nrow (`{0} \x `[0, Ncol])) //.
+  set (R1 (i : Dom) := arr(x_mval, mval)⟨2, i⟩ \*
+    arr(x_colind, colind)⟨2, i⟩ \* 
+    arr(x_rowptr, rowptr)⟨2, i⟩).
+  set (R2 (i : Dom) := arr(y_ind, yind)⟨3, i⟩ \*
+    arr(y_val, yval)⟨3, i⟩).
+  set (Inv (i : int) := arr(x_mval, mval)⟨1, (0,0)⟩ \* 
+    arr(x_colind, colind)⟨1, (0,0)⟩ \* 
+    arr(x_rowptr, rowptr)⟨1, (0,0)⟩ \*
+    arr(y_ind, yind)⟨1, (0,0)⟩ \* 
+    arr(y_val, yval)⟨1, (0,0)⟩).
+  xfor_specialized_normal2 Inv R1 R1 R2 R2 
+    (fun hv i => Σ_(j <- `{i} \x `[0, Ncol]) (hv[`2](j) * hv[`3]((0, j.2))))
+    (fun=> 0) s.
+  { xin (2,0) : rewrite wp_prod_single /=.
+    xin (1,0) : do 3 (xwp; xapp)...
+    xframe2 (arr(x_rowptr, rowptr)⟨1, (0, 0)⟩).
+    xsubst (snd : _ -> int).
+    xnapp @sv.sv_dotprod_spec... 
+    { by rewrite -len_xind /slice slice_fullE. }
+    { move=> ? /in_interval_list... }
+    { move=> ?; rewrite -len_xind /slice slice_fullE... }
+    move=> ?; rewrite -wp_equiv. xsimpl=>->.
+    xapp @lhtriple_array_set_pre; try math.
+    rewrite sum_prod1E; xsimpl. }
+  { rewrite Union_same //; xsimpl*. }
+  xwp; xval. xsimpl*. xsimpl; rewrite sum_prod1E; xsimpl.
 Qed.
 
 End csr.
