ListCommon.v
@@ -1,0 +1,132 @@
+From mathcomp Require Import seq ssrbool eqtype choice.
+From SLF Require Import Sum Fun LabType Unary_IndexWithBounds.
+
+Import List.
+
+Definition sorted (l : list int) : Prop. Admitted.
+Definition max (l : list int) : int. Admitted.
+
+Definition merge (l1 l2 : list int) : list int. Admitted.
+
+Lemma In_merge l1 l2 x : In x (merge l1 l2) = (In x l1 \/ In x l2).
+Proof. Admitted.
+
+Lemma sorted_nodup l : sorted l -> NoDup l.
+Admitted.
+
+Lemma sorted_merge l1 l2 : sorted l1 -> sorted l2 -> sorted (merge l1 l2).
+Admitted.
+
+Lemma sorted_max_size l i : 
+  i + 1 = length l -> l[i] = max l.
+Admitted.
+
+Lemma max_sublist l1 l2 : 
+  (forall x, In x l1 -> In x l2) -> max l2 >= max l1.
+Admitted.
+
+Lemma nth_le_max l i :
+  i >= 0 ->
+  sorted l ->
+  l[i] >= max l -> i + 1 = length l.
+Admitted.
+
+Lemma sorted_le i j l :
+  sorted l ->
+  0 <= i < length l ->
+  0 <= j < length l ->
+    i < j -> l[i] < l[j].
+Admitted.
+
+Lemma max_takeS i l : 
+  0 <= i < length l ->
+  max (take (abs (i + 1)) l) = Z.max l[i] (max (take (abs i) l)).
+Admitted.
+
+Lemma In_lt x i l :
+  0 <= i < length l - 1 ->
+  sorted l ->
+    In x l -> x < l[i+1] -> x <= l[i].
+Admitted.
+
+Lemma max_le x l : 
+  In x l -> x <= max l.
+Proof.
+Admitted.
+
+Lemma size_merge l1 l2: 
+  length (merge l1 l2) >= Z.max (length l1) (length l2).
+Proof.
+Admitted.
+
+Lemma max0 : max nil = -1.
+Proof.
+Admitted.
+
+Lemma In_le_0 l x :
+  sorted l -> In x l -> x >= l[0].
+Admitted.
+
+Lemma search (x : int) (l : list int) : int.
+Admitted. (*find 0 (> x)*)
+
+Lemma search_lt_nth l i x : 
+  sorted l -> 
+  0 <= i < length l ->
+    (forall y, In y l -> y < l[i] -> y <= x) ->
+    x < l[i] ->
+    search x l = l[i].
+Admitted.
+
+Lemma search_nth l i : 
+  sorted l -> 
+  0 < i + 1 < length l ->
+    search l[i] l = l[i + 1].
+Admitted.
+
+Lemma merge_nthS l1 l2 i :
+  sorted l1 -> sorted l2 ->
+  0 < i + 1 < length (merge l1 l2) ->
+    (merge l1 l2)[i+1] = Z.min (search (merge l1 l2)[i] l1) (search (merge l1 l2)[i] l2).
+Admitted.
+
+Lemma merge_nth0 l1 l2 :
+  length l1 > 0 ->
+  length l2 > 0 ->
+  (merge l1 l2)[0] = Z.min l1[0] l2[0].
+Admitted.
+
+Lemma NoDup_nthZ {A : Type} i j l (z : A): 
+  NoDup l <->
+  ((0<= i < Datatypes.length l) ->
+  (0<= j < Datatypes.length l) -> nth (abs i) l z = nth (abs j) l z -> i = j).
+Admitted.
+
+Lemma in_combineE {A B : Type} (l : list A) (l' : list B) (x : A) (y : B) :
+  In (x, y) (combine l l') = (In x l /\ In y l').
+Admitted.
+
+Fact Sum_list_interval  (f : int -> int) (a b : int) l:
+  NoDup (list_interval (abs a) (abs b) l) ->
+  Sum (list_interval (abs a) (abs b) l) f = 
+  Sum `[a, b] (fun i => f l[i]).
+Admitted.
+
+Fact intr_list (a b : int) (l: list int) : 
+  (forall x, In x l -> a <= x < b) ->
+  `[a, b] ∩ l = l.
+Admitted.
+
+Lemma slice_fullE {A : Type} (l : list A) : 
+  list_interval (abs 0) (abs (length l)) l = l.
+Admitted.
+
+Lemma Union_same {B C} (v : int) (f : fmap B C) : 
+  v > 0 -> 
+    Union `[0, v] (fun _ => f) = f.
+Admitted.
+
+Lemma in_interval_list {A : Type} (l : list A) lb rb x: 
+   In x (list_interval lb rb l) -> In x l.
+Proof.
+Admitted.
