Loops.v
@@ -1358,7 +1358,7 @@ Lemma xfor_lemma2_hbig_op `{ID : Inhab D}
     {{ v, 
         Inv (l + 1) \* 
         (\*_(d <- ⟨(j,0)%Z, fsi1 l⟩) R1' d) \* 
-        (\*_(d <- ⟨(j,0)%Z, fsi2 l⟩) R2' d) \* 
+        (\*_(d <- ⟨(k,0)%Z, fsi2 l⟩) R2' d) \* 
         Q \(m, vd) H' l v }}) ->
   (forall j : int, hlocal (Inv j) ⟨(i,0%Z), single s tt⟩) ->
   (forall j : int, hlocal (H j) ⟨(i,0%Z), single s tt⟩) ->
@@ -1785,7 +1785,7 @@ Lemma xfor_lemma_gen2_bigstr `{ID : Inhab D}
     {{ v, 
         Inv (l + 1) \* 
         (\*_(d <- ⟨(j,0)%Z, fsi1 l⟩) R1' d) \* 
-        (\*_(d <- ⟨(j,0)%Z, fsi2 l⟩) R2' d) \* 
+        (\*_(d <- ⟨(k,0)%Z, fsi2 l⟩) R2' d) \* 
         H' l v }}) ->
   (forall j : int, hlocal (Inv j) ⟨(i,0%Z), single s tt⟩) ->
   (forall j : int, hlocal (H j) ⟨(i,0%Z), single s tt⟩) ->
@@ -1904,18 +1904,22 @@ Qed.
 Lemma xfor_lemma_gen2_array `{ID : Inhab D}
   Inv 
   (R1 R1' R2 R2' : Dom -> hhprop)
-  s fsi1 fsi2 vr (arrl : loc) (arr1 : list int) arr2
-  (N: Z) (C1 C2 : Dom -> trm) (C : trm)
+  s fsi1 fsi2 vr (arrl : loc) (arr1 : list int) arr2 idx
+  (N M : Z) (C1 C2 : Dom -> trm) (C : trm)
   (i j k : Z)
   Pre Post: 
-  (forall v, length (arr2 v) = N :> int) ->
-  length arr1 = N :> int ->
+  (forall v, length (arr2 v) = M :> int) ->
+  length arr1 = M :> int ->
+  length idx = N :> int ->
+  NoDup idx ->
+  (forall (l : int), 
+    (0 <= l < N) -> 0 <= idx[l] < M) ->
   (forall (l : int), 
     (0 <= l < N) ->
     {{ Inv l \* 
         (\*_(d <- ⟨(j,0)%Z, fsi1 l⟩) R1 d) \* 
         (\*_(d <- ⟨(k,0)%Z, fsi2 l⟩) R2 d) \* 
-        (arrl + 1 + abs l)%nat ~⟨(i,0)%Z, s⟩~> arr1[l] }}
+        (arrl + 1 + abs idx[l])%nat ~⟨(i,0)%Z, s⟩~> arr1[idx[l] ] }}
       [{
         {i| _  in single s tt  => subst vr l C};
         {j| ld in fsi1 l       => C1 ld};
@@ -1924,8 +1928,8 @@ Lemma xfor_lemma_gen2_array `{ID : Inhab D}
     {{ v, 
         Inv (l + 1) \* 
         (\*_(d <- ⟨(j,0)%Z, fsi1 l⟩) R1' d) \* 
-        (\*_(d <- ⟨(j,0)%Z, fsi2 l⟩) R2' d) \* 
-        (arrl + 1 + abs l)%nat ~⟨(i,0)%Z, s⟩~> (arr2 v)[l] }}) ->
+        (\*_(d <- ⟨(k,0)%Z, fsi2 l⟩) R2' d) \* 
+        (arrl + 1 + abs idx[l])%nat ~⟨(i,0)%Z, s⟩~> (arr2 v)[idx[l] ] }}) ->
   (forall j : int, hlocal (Inv j) ⟨(i,0%Z), single s tt⟩) ->
   (forall i : Dom, hlocal (R1 i) ⟨(j,0%Z), single i tt⟩) ->
   (forall i : Dom, hlocal (R1' i) ⟨(j,0%Z), single i tt⟩) ->
@@ -1935,7 +1939,9 @@ Lemma xfor_lemma_gen2_array `{ID : Inhab D}
     0 <= m < N ->
     (forall i, indom (fsi1 m) i -> hv[`j](i) = hv'[`j](i)) ->
     (forall i, indom (fsi2 m) i -> hv[`k](i) = hv'[`k](i)) ->
-    (arr2 hv)[m] = (arr2 hv')[m]) ->
+    (arr2 hv)[idx[m] ] = (arr2 hv')[idx[m] ]) ->
+  (forall (hv : D -> val) m,
+    0 <= m < M -> ~ In m idx -> arr1[m] = (arr2 hv)[m]) ->
   (i <> j)%Z ->
   (j <> k)%Z ->
   (k <> i)%Z ->
@@ -1965,9 +1971,12 @@ Lemma xfor_lemma_gen2_array `{ID : Inhab D}
     }]
   {{ v, Post v }}. 
 Proof.
-  move=> AL1 AL2 IH ????? hvE ?????????? PreH PostH.
+  move=>  AL1 AL2 ALidx Hnodup Hidx IH ????? hvE Hpre ????????? PreH PostH.
   have AL : forall hv, Datatypes.length arr1 = Datatypes.length (arr2 hv).
   { move=> v; move: (AL1 v). lia. }
+  have Hidx' : forall x : int, In x idx -> 0 <= x < M.
+  { intros. eapply In_nth with (d:=0) in H. destruct H as (n & Hn & <-). 
+    replace n with (abs n)%nat by math. apply Hidx. math. }
   apply/ntriple_conseq; last exact/PostH; eauto.
   rewrite /harray_int/harray/hheader ?length_map ?length_List_length.
   apply/(ntriple_conseq); [|exact: himpl_trans|move=> ?]; first last.
@@ -1975,16 +1984,35 @@ Proof.
     move=> ?; apply:applys_eq_init; reflexivity. }
   xframe2 (arrl ~⟨(i, 0%Z), s⟩~> val_header (length arr1)).
   xframe2 \[(arrl, (⟨(i, 0), s⟩)%arr) <> null (⟨(i, 0), s⟩)%arr].
-  rewrite ?hcellsE.  
+  rewrite ?hcellsE AL2.
+  rewrite -> hbig_fset_part with (fs:=`[0, M]) (P:=idx).
+  set (Inv' := hbig_fset _ (_ ∖ _) _).
+  rewrite intr_list // (fset_of_list_nodup 0) // ALidx hbig_fset_Union.
+  2:{ introv Ha Hb Hc. apply disjoint_single_single. intros Hd. rewrite ! indom_interval in Hb, Hc. apply Ha. enough (abs i0 = abs j0) by lia.
+    move: Hd. erewrite -> NoDup_nth in Hnodup. apply Hnodup; math. }
   eapply xfor_lemma_gen2_bigstr with 
-  (H := fun l => (arrl + 1 + abs l)%nat ~⟨(i, 0%Z), s⟩~> arr1[l])
-  (H' := fun l v => (arrl + 1 + abs l)%nat ~⟨(i, 0%Z), s⟩~> (arr2 v)[l])
+  (Inv := fun i => Inv i \* Inv')
+  (H := fun l => (arrl + 1 + abs idx[l])%nat ~⟨(i, 0%Z), s⟩~> arr1[idx[l] ])
+  (H' := fun l v => (arrl + 1 + abs idx[l])%nat ~⟨(i, 0%Z), s⟩~> (arr2 v)[idx[l] ])
   (R1 := R1) (R2 := R2) (R2' := R2') (R1' := R1'); try eassumption; autos*=> //.
+  { move=> l Hl. xframe2 Inv'. rewrite wp_equiv. eapply htriple_conseq. 1: apply wp_equiv, IH=> //. all: xsimpl*. 
+    (* xnsimpl will make over simplification *) }
+  { rewrite /Inv'. xlocal. autos*.
+    apply/hlocal_hstar_fset=> ??. apply/hlocal_hsingle.
+    by rewrite indom_label_eq indom_single_eq. }
   { xlocal. }
   { xlocal. }
   { move=> ???? hvE1 hvE2; erewrite hvE; eauto. }
-  { rewrite AL2. xsimpl. }
-  move=> ?. rewrite hcellsE AL1. xsimpl*.
+  { xsimpl*=> ?; apply:applys_eq_init. f_equal. extens=> ?. 
+   by rewrite hstar_fset_label_single. }
+  move=> ?. rewrite /Inv' hcellsE AL1 !fun_eta_1. xsimpl*. 
+  rewrite -> hbig_fset_part with (fs:=`[0, M]) (P:=idx).
+  rewrite intr_list // (fset_of_list_nodup 0) // ALidx hbig_fset_Union.
+  2:{ introv Ha Hb Hc. apply disjoint_single_single. intros Hd. rewrite ! indom_interval in Hb, Hc. apply Ha. enough (abs i0 = abs j0) by lia.
+    move: Hd. erewrite -> NoDup_nth in Hnodup. apply Hnodup; math. }
+  erewrite hbig_fset_eq with (fs:=`[0, N]). 1: xsimpl*. 2: move=> * /=; by rewrite hbig_fset_label_single'.
+  erewrite hbig_fset_eq. 1: xsimpl*. 
+  move=> d Hnotin /=. rewrite filter_indom indom_interval /Sum.mem /= in Hnotin. do 2 f_equal. now apply Hpre.
 Qed.
 
 Lemma xfor_lemma_gen_array `{ID : Inhab D}
@@ -2174,3 +2202,31 @@ Ltac xwhile1 Z N b Inv :=
   let Inv' := constr:(Inv) in
   xseq_xlet_if_needed; xstruct_if_needed;
   eapply (wp_while_unary Inv b (Z := Z) (N := N)); autos*.
+
+Tactic Notation "xwhile_sum" 
+    constr(Inv) 
+    constr(R1) constr(R2) 
+    uconstr(R1') uconstr(R2') 
+    constr(op) constr(s) :=
+  eapply (@xwhile_big_op_lemma2 _ _
+    Inv R1 R2 R1' R2' op s)=> //;
+  [
+  |
+  |
+  | intro; rewrite ?/Inv; xsimpl*
+  | disjointE
+  | disjointE 
+  | let hvE1 := fresh "hvE1" in
+    let hvE2 := fresh "hvE2" in
+    let someindom := fresh "someindom" in
+    intros ??? hvE1 hvE2; rewrite ?/op;
+    match goal with 
+    | |- Sum ?a _ = Sum ?a _ => apply fold_fset_eq; intros ? someindom; extens; intros 
+    | _ => idtac
+    end; try setoid_rewrite hvE1; try setoid_rewrite hvE2 
+    (**; [eauto|autorewrite with indomE; try math; 
+    (first [ apply someindom | idtac ])]*)
+  | try lia
+  |
+  |
+  ].
